src/program_proof/rsm/distx/invariance/read.v
@@ -1,0 +1,190 @@
+From Perennial.program_proof.rsm.distx Require Import prelude.
+
+Lemma ext_by_cmtd_inv_read {repl cmtd kmodc} tid tsprep :
+  (tid ≤ length repl)%nat ->
+  cmtd ≠ [] ->
+  ext_by_cmtd repl cmtd kmodc tsprep ->
+  ext_by_cmtd repl (last_extend tid cmtd) kmodc tsprep.
+Proof.
+  rewrite /ext_by_cmtd.
+  intros Hlenr Hnnil Hext.
+  destruct (kmodc !! tsprep) as [v |].
+  - destruct (decide (tid ≤ length cmtd)%nat) as [Hlenc | Hlenc].
+    { by rewrite last_extend_id; last apply Hlenc. }
+    rewrite Nat.nle_gt in Hlenc.
+    assert (Hlen : (length repl < length cmtd)%nat).
+    { rewrite Hext.
+      rewrite length_app /=.
+      pose proof (last_extend_length_ge tsprep repl) as Hlen.
+      lia.
+    }
+    lia.
+  - destruct Hext as [Hext Htsprep].
+    split; last apply Htsprep.
+    destruct Hext as [tsr Hext].
+    destruct (decide (tsr ≤ length cmtd)%nat) as [Hlenc | Hlenc].
+    + (* we have [repl = cmtd] from [Hext Hlenc] *)
+      rewrite last_extend_id in Hext; last apply Hlenc. subst repl.
+      exists O.
+      by rewrite last_extend_twice /= last_extend_id.
+    + rewrite Nat.nle_gt in Hlenc.
+      assert (Hlen : length repl = tsr).
+      { rewrite Hext last_extend_length_eq_n; [done | done | lia]. }
+      rewrite Hlen in Hlenr.
+      exists tsr.
+      rewrite last_extend_twice.
+      by replace (_ `max` _)%nat with tsr by lia.
+Qed.
+
+Lemma head_read_first_commit_compatible future ts tshd wrs keyhd :
+  head_read future tshd keyhd ->
+  first_commit_compatible future ts wrs ->
+  keyhd ∈ dom wrs ->
+  (tshd ≤ ts)%nat.
+Proof.
+  intros Hhr (lp & ls & (Happ & _ & Hhead) & Hcomp) Hnempty.
+  destruct (decide (lp = [])) as [-> | Hnnil].
+  { rewrite Happ /= /head_read Hhead in Hhr. inv Hhr. }
+  assert (Hlp : ActRead tshd keyhd ∈ lp).
+  { apply head_Some_elem_of.
+    rewrite (head_prefix _ future); [done | apply Hnnil |].
+    rewrite Happ.
+    by apply prefix_app_r.
+  }
+  rewrite /compatible_all Forall_forall in Hcomp.
+  specialize (Hcomp _ Hlp).
+  destruct Hcomp; [lia | contradiction].
+Qed.
+
+Lemma conflict_free_inv_read {future tmodcs tid key} :
+  head_read future tid key ->
+  conflict_free future tmodcs ->
+  conflict_free (tail future) tmodcs.
+Proof.
+  intros Hhead Hcf ts wrs Hwrs.
+  specialize (Hcf _ _ Hwrs). simpl in Hcf.
+  by unshelve eapply (first_commit_compatible_inv_tail_future _ _ _ _ _ Hhead).
+Qed.
+
+Lemma conflict_past_inv_read {past future tmodas tid key} :
+  head_read future tid key ->
+  conflict_past past future tmodas ->
+  conflict_past (past ++ [ActRead tid key]) (tail future) tmodas.
+Proof.
+  intros Hhead Hcp ts form Hform.
+  specialize (Hcp _ _ Hform). simpl in Hcp.
+  rewrite /conflict_cases in Hcp.
+  destruct form as [| wrsx | wrsx]; simpl.
+  - by apply no_commit_inv_tail_future.
+  - by apply first_commit_incompatible_inv_snoc_past_tail_future.
+  - by unshelve eapply (first_commit_compatible_inv_tail_future _ _ _ _ _ Hhead).
+Qed.
+
+Lemma cmtxn_in_past_inv_read {past resm} tid key :
+  cmtxn_in_past past resm ->
+  cmtxn_in_past (past ++ [ActRead tid key]) resm.
+Proof.
+  intros Hcmtxn ts wrs Hwrs.
+  specialize (Hcmtxn _ _ Hwrs). simpl in Hcmtxn.
+  set_solver.
+Qed.
+
+Section inv.
+  Context `{!distx_ghostG Σ}.
+
+  Lemma key_inv_read γ kmodl tid key vl vr :
+    tid ≠ O ->
+    le_all tid (dom kmodl) ->
+    hist_lnrz_at γ key (pred tid) vl -∗
+    hist_repl_at γ key (pred tid) vr -∗
+    key_inv_with_kmodl γ key kmodl ==∗
+    key_inv_with_kmodl γ key kmodl ∗
+    hist_cmtd_length_lb γ key tid ∗
+    ⌜vl = vr⌝.
+  Proof.
+    iIntros (Hnz Hleall) "#Hlnrzlb #Hrepllb Hkey".
+    iNamed "Hkey". iNamed "Hprop".
+    (* Obtain value at [pred tid] for both [cmtd] and [lnrz]. *)
+    iDestruct (hist_lnrz_lookup with "Hlnrz Hlnrzlb") as %Hvl.
+    iDestruct (hist_repl_lookup with "Hrepl Hrepllb") as %Hvr.
+    (* Re-establish [ext_by_lnrz] and [ext_by_cmtd]. *)
+    assert (Hlenl : (tid ≤ length lnrz)%nat).
+    { apply lookup_lt_Some in Hvl. lia. }
+    pose proof (ext_by_lnrz_inv_read _ _ _ _ Hlenl Hleall Hdiffl) as Hdiffl'.
+    assert (Hlenr : (tid ≤ length repl)%nat).
+    { apply lookup_lt_Some in Hvr. lia. }
+    pose proof (ext_by_lnrz_not_nil _ _ _ Hdiffl) as Hnnil.
+    pose proof (ext_by_cmtd_inv_read tid _ Hlenr Hnnil Hdiffc) as Hdiffc'.
+    (* Extend [hist_cmtd_auth] to [tid]. Note that it's a no-op when [tid ≤ length cmtd]. *)
+    set cmtd' := last_extend _ _ in Hdiffl' Hdiffc'.
+    iMod (hist_cmtd_update cmtd' with "Hcmtd") as "Hcmtd".
+    { apply last_extend_prefix. }
+    iAssert (hist_cmtd_length_lb γ key tid)%I as "#Hlb".
+    { iDestruct (hist_cmtd_witness with "Hcmtd") as "#Hlb".
+      iFrame "Hlb".
+      iPureIntro.
+      by apply last_extend_length_ge_n.
+    }
+    assert (Heq : vl = vr).
+    { (* Obtain [prefix cmtd' lnrz]. *)
+      destruct Hdiffl' as (_ & Hprefixcl & _).
+      assert (Hlenc : (pred tid < length cmtd')%nat).
+      { assert (Hlenc : (tid ≤ length cmtd')%nat); first by apply last_extend_length_ge_n. lia. }
+      pose proof (prefix_lookup_lt _ _ _ Hlenc Hprefixcl) as Hvl'.
+      rewrite Hvl in Hvl'.
+      pose proof (ext_by_cmtd_prefix Hdiffc') as Hprefix.
+      destruct Hprefix as [Hprefixrc | Hprefixcr].
+      { pose proof (prefix_lookup_Some _ _ _ _ Hvr Hprefixrc) as Hvr'.
+        rewrite Hvl' in Hvr'.
+        by inv Hvr'.
+      }
+      { pose proof (prefix_lookup_lt _ _ _ Hlenc Hprefixcr) as Hvr'.
+        rewrite Hvr Hvl' in Hvr'.
+        by inv Hvr'.
+      }
+    }
+    by iFrame "∗ # %".
+  Qed.
+
+  Lemma txn_inv_read γ tid key vl vr future :
+    tid ≠ O ->
+    head_read future tid key ->
+    hist_lnrz_at γ key (pred tid) vl -∗
+    hist_repl_at γ key (pred tid) vr -∗
+    txn_inv_no_future γ future -∗
+    key_inv γ key ==∗
+    txn_inv_no_future γ (tail future) ∗
+    key_inv γ key ∗
+    ⌜vl = vr⌝.
+  Proof.
+    iIntros (Hnz Hhead) "#Hlnrzlb #Hrepllb Htxn Hkey".
+    iNamed "Htxn".
+    iDestruct (key_inv_expose_kmodl with "Hkey") as (kmodl) "Hkey".
+    iAssert (⌜le_all tid (dom kmodl)⌝)%I as %Hleall.
+    { iNamed "Hkey". iNamed "Hprop".
+      iDestruct (big_sepS_elem_of _ _ key with "Hkmodls") as "Hkmodl'".
+      { apply Hall. }
+      iDestruct (kmod_lnrz_agree with "Hkmodl' Hkmodl") as %->.
+      iPureIntro.
+      intros tsx Htsx.
+      apply elem_of_dom_vslice in Htsx as [wrs [Hwrs Hinwrs]].
+      specialize (Hcf _ _ Hwrs). simpl in Hcf.
+      eapply head_read_first_commit_compatible; [apply Hhead | apply Hcf | apply Hinwrs].
+    }
+    (* Obtain a witness that the committed history has been extended to [tid], and [vl = vr]. *)
+    iMod (key_inv_read with "Hlnrzlb Hrepllb Hkey") as "(Hkey & #Hcmtd & %Heq)".
+    { apply Hnz. }
+    { apply Hleall. }
+    iDestruct (key_inv_hide_kmodl with "Hkey") as "Hkey".
+    (* Re-establish [past_action_witness]. *)
+    iAssert (past_action_witness γ (ActRead tid key))%I as "#Hpa"; first iFrame "Hcmtd".
+    iCombine "Hpas Hpa" as "Hpas'".
+    rewrite -big_sepL_snoc.
+    (* Re-establish [conflict_free], [conflict_past], [cmtxn_in_past] w.r.t. read. *)
+    pose proof (conflict_free_inv_read Hhead Hcf) as Hcf'.
+    pose proof (conflict_past_inv_read Hhead Hcp) as Hcp'.
+    pose proof (cmtxn_in_past_inv_read tid key Hcmtxn) as Hcmtxn'.
+    by iFrame "∗ # %".
+  Qed.
+
+End inv.
